add lemma proving that specific sigmas on 10.4.3 unify a term.

B_Unification/lowenheim_proof.v
@@ -160,3 +160,191 @@ Proof.
     + pose helper_2a as H2. specialize (H2 t1 t2 t'). apply H2. apply H. 
 Qed.
 
+
+
+(** 3.1 Declarations useful for the proof **)
+
+
+Axiom refl_comm :
+  forall t1 t2, t1 == t2 -> t2 == t1.
+
+Lemma subst_distr_opp :
+  forall s x y, apply_subst (x + y) s == apply_subst x s + apply_subst y s.
+Proof.
+  intros.
+  apply refl_comm.
+  apply subst_distribution.
+Qed. 
+
+
+Lemma subst_mul_distr_opp :
+  forall s x y, apply_subst (x * y) s == apply_subst x s * apply_subst y s.
+Proof.
+  intros.
+  apply refl_comm.
+  apply subst_associative.
+Qed. 
+
+
+Lemma sum_assoc_opp :
+ forall x y z, x + (y + z) == (x + y) + z.
+Proof.
+Admitted.
+
+Lemma mul_assoc_opp :
+ forall x y z, x * (y * z) == (x * y) * z.
+Proof.
+Admitted.
+
+
+Lemma var_subst:
+  forall (v : var) (ts : term) ,
+  (apply_subst (VAR v) (cons (v , ts) nil) ) == ts.
+Proof.
+Admitted.
+
+Lemma id_subst:
+  forall (t : term) (x : var),
+  apply_subst t [(x , VAR x)] == t.
+Proof.
+Admitted.
+
+   
+
+
+
+
+
+
+Definition sub_term (t : term) (t' : term) : Prop :=
+  forall (x : var ),
+  (In x (term_unique_vars t) ) -> (In x (term_unique_vars t')) .
+
+Lemma sub_term_v :
+  forall (v : var),
+  sub_term (VAR v) (VAR v).
+ Proof.
+Admitted.
+
+Lemma sub_term_id :
+  forall (t : term),
+  sub_term t t.
+ Proof.
+Admitted.
+
+Fixpoint build_on_list_of_vars (list_var : var_set) (s : term) (sig1 : subst) (sig2 : subst) : subst :=
+  match list_var with 
+   | nil => nil 
+   | v' :: v =>
+      (cons (v' , (s + T1) * (apply_subst (VAR v') sig1 )  + s * (apply_subst (VAR v' ) sig2 )  )    
+            (build_on_list_of_vars v s sig1 sig2) )
+  end. 
+
+
+Lemma helper_1:
+forall (t' s : term) (v : var) (sig1 sig2 : subst),
+  sub_term (VAR v) t' -> 
+  apply_subst (VAR v) (build_on_list_of_vars (term_unique_vars t') s sig1 sig2)
+  == 
+  apply_subst (VAR v) (build_on_list_of_vars (term_unique_vars (VAR v)) s sig1 sig2).
+Proof.
+Admitted.
+
+Lemma helper_2a:
+  forall (t1 t2 t' : term),
+  sub_term (t1 + t2) t' -> sub_term t1 t'.
+Proof.
+Admitted. 
+  
+Lemma helper_2b:
+  forall (t1 t2 t' : term),
+  sub_term (t1 + t2) t' -> sub_term t2 t'.
+Proof.
+Admitted. 
+
+
+
+
+
+(* Lemma 10.4.3*)
+
+Lemma subs_distr_vars_ver2 :
+  forall (t t' : term) (s : term) (sig1 sig2 : subst),
+  (sub_term t t') ->
+  apply_subst t (build_on_list_of_vars  (term_unique_vars t') s sig1 sig2)
+    ==
+  (s + T1) * (apply_subst t sig1) + s * (apply_subst t sig2).
+Proof.
+ intros. generalize dependent t'.  induction t.
+  - intros t'. repeat rewrite ground_term_cannot_subst.
+    + rewrite mul_comm with (x := s + T1). rewrite distr. repeat rewrite mul_T0_x. rewrite mul_comm with (x := s).
+      rewrite mul_T0_x.  repeat rewrite sum_x_x. reflexivity.
+    + unfold ground_term. reflexivity.
+    + unfold ground_term. reflexivity.
+    + unfold ground_term. reflexivity.
+  - intros t'. repeat rewrite ground_term_cannot_subst.
+    + rewrite mul_comm with (x := s + T1). rewrite mul_id. rewrite mul_comm with (x := s). rewrite mul_id. rewrite sum_comm with (x := s).
+      repeat rewrite sum_assoc. rewrite sum_x_x.  rewrite sum_comm with (x := T1). rewrite sum_id. reflexivity.
+    +  unfold ground_term. reflexivity.
+    +  unfold ground_term. reflexivity.
+    + unfold ground_term. reflexivity.
+  - intros. rewrite helper_1 .
+    + unfold term_unique_vars. unfold term_vars. unfold var_set_create_unique. unfold var_set_includes_var. unfold build_on_list_of_vars.
+    rewrite var_subst. reflexivity. 
+    + apply H. 
+  -  intros. specialize (IHt1 t'). specialize (IHt2 t').  repeat rewrite subst_distr_opp. 
+      rewrite IHt1. rewrite IHt2.
+    + rewrite distr. rewrite distr. repeat rewrite sum_assoc. rewrite sum_comm with (x := (s + T1) * apply_subst t2 sig1)
+      (y := (s * apply_subst t1 sig2 + s * apply_subst t2 sig2)). repeat rewrite sum_assoc.
+      rewrite sum_comm with (x := s * apply_subst t2 sig2 ) (y := (s + T1) * apply_subst t2 sig1).
+      repeat rewrite sum_assoc. reflexivity.
+    + pose helper_2b as H2. specialize (H2 t1 t2 t'). apply H2. apply H. 
+    + pose helper_2a as H2. specialize (H2 t1 t2 t'). apply H2. apply H. 
+  - intros. specialize (IHt1 t'). specialize (IHt2 t'). repeat rewrite subst_mul_distr_opp. rewrite IHt1. rewrite IHt2.
+    + rewrite distr. rewrite mul_comm with (y := ((s + T1) * apply_subst t2 sig1)).
+    rewrite distr. rewrite mul_comm with (y := (s * apply_subst t2 sig2)). rewrite distr.
+    repeat rewrite mul_assoc. repeat rewrite mul_comm with (x := apply_subst t2 sig1).
+    repeat rewrite mul_assoc.
+    rewrite mul_assoc_opp with (x := (s + T1)) (y := (s + T1)) . rewrite mul_x_x.
+    rewrite mul_assoc_opp with (x := (s + T1)) (y := s). rewrite mul_comm with (x := (s + T1)) (y := s).
+    rewrite distr. rewrite mul_x_x. rewrite mul_id_sym. rewrite sum_x_x. rewrite mul_T0_x.
+    repeat rewrite mul_assoc. rewrite mul_comm with (x := apply_subst t2 sig2 ).
+    repeat rewrite mul_assoc. rewrite mul_assoc_opp with (x := s ) (y := (s + T1)).
+    rewrite distr. rewrite mul_x_x. rewrite mul_id_sym. rewrite sum_x_x. rewrite mul_T0_x.
+    repeat rewrite sum_assoc. rewrite sum_assoc_opp with (x := T0) (y := T0). rewrite sum_x_x. rewrite sum_id.
+    repeat rewrite mul_assoc. rewrite mul_comm with (x := apply_subst t2 sig2) (y := s * apply_subst t1 sig2).
+    repeat rewrite mul_assoc. rewrite mul_assoc_opp with (x := s). rewrite mul_x_x. reflexivity.
+    + pose helper_2b as H2. specialize (H2 t1 t2 t'). apply H2. apply H. 
+    + pose helper_2a as H2. specialize (H2 t1 t2 t'). apply H2. apply H. 
+Qed.
+
+Lemma specific_sigmas_unify:
+  forall (t : term) (tau : subst) (x : var),
+  (unifier t tau) -> 
+  (apply_subst t (build_on_list_of_vars  (term_unique_vars t) t (cons (x , (VAR x)) nil ) tau )
+  ) == T0 .
+  Proof.
+  intros. 
+  rewrite subs_distr_vars_ver2.
+  + rewrite id_subst. rewrite mul_comm with (x := t + T1). rewrite distr. rewrite mul_x_x. rewrite mul_id_sym. rewrite sum_x_x.
+    rewrite sum_id. 
+    unfold unifier in H. rewrite H. rewrite mul_T0_x_sym. reflexivity.
+  +  apply sub_term_id.
+Qed.
+
+Definition eqv_lists {A : Type} (l1 : list A) (l2 : list A) : Prop :=
+forall (elt : A),
+ In elt l1 <-> In elt l2.
+     
+Lemma specific_sigmas_is_lowengeim:
+forall (t : term) (tau : subst) (x : var),
+ (unifier t tau) ->
+  eqv_lists
+(build_on_list_of_vars  (term_unique_vars t) t (cons (x , (VAR x)) nil ) tau )
+( lowenheim_subst t tau).
+Proof.
+intros. unfold eqv_lists. intros.
+split.
+ - induction t.
+   + 
+Admitted.
